ROOT
@@ -1,18 +1,16 @@
-session "IsaCrypt" = "IsaCrypt-Prereqs" +
+session "IsaCrypt" = "HOL-Probability" + 
   options [document = pdf, quick_and_dirty = true, (*z3_non_commercial = yes,*) document_output = "output", browser_info = true]
+  sessions "HOL-Nominal" "HOL-Proofs-Lambda" "HOL-ZF"
   theories [document = false]
   theories (*ISACRYPT_THYS*) Distr ElGamal Hoare_Tactics Hoare_Typed Hoare_Untyped Lang_Simplifier Lang_Typed Lang_Untyped Misc Procedures Procs_Typed RHL_Typed RHL_Untyped Tactic_Inline TermX_Antiquot Tools TypedLambda TypedLambdaNominal Universe
   document_files (in ".")
     "root.tex"
 
-session "IsaCrypt-Nodocs" = "IsaCrypt-Prereqs" +
-  options [document = false, quick_and_dirty = true]
-  theories [document = false]
-  theories (*ISACRYPT_THYS*) Distr ElGamal Hoare_Tactics Hoare_Typed Hoare_Untyped Lang_Simplifier Lang_Typed Lang_Untyped Misc Procedures Procs_Typed RHL_Typed RHL_Untyped Tactic_Inline TermX_Antiquot Tools TypedLambda TypedLambdaNominal Universe
-  document_files (in ".")
-    "root.tex"
+session "IsaCrypt-Prereqs" = "HOL-Probability" +
+  sessions "HOL-Nominal" "HOL-Proofs-Lambda" "HOL-ZF"
+  theories [document = false] Prereqs
 
-
+(*
 session "IsaCrypt-Prereqs" in "~~/src/HOL" = "HOL-Analysis" +
   description {*
     Prerequisites for running the IsaCrypt theories.
@@ -26,16 +24,4 @@ session "IsaCrypt-Prereqs" in "~~/src/HOL" = "HOL-Analysis" +
     "Proofs/Lambda/ListOrder"
     "Library/Rewrite"
     "Nominal/Nominal"
-
-session "IsaCrypt-Core" = "IsaCrypt-Prereqs" +
-  description {*
-    Partial IsaCrypt heap
-  *}
-  theories Universe Tools Distr Lang_Untyped TypedLambda TermX_Antiquot
-
-session "IsaCrypt-Prereqs-Proofs" = "IsaCrypt-Prereqs" +
-  theories "~~/src/HOL/Proofs"
-
-session "IsaCrypt-Print-Sorry" = "IsaCrypt-Prereqs-Proofs" +
-  options [(*z3_non_commercial = yes, *) quick_and_dirty = false]
-  theories Tmp_Print_Sorry
+*)
